theories/logrel/logrel.v
@@ -17,7 +17,7 @@ Section logrel.
 
   (* XXX: a better def using list zip? - no, gmap makes case analysis simpler*)
   Definition unknown_mem_page (p: PID) :=
-    (∃ mem, ⌜dom (gset Addr) mem = list_to_set (addr_of_page p)⌝ ∗ [∗ map] a ↦ w ∈ mem, (a ->a w))%I.
+    (∃ mem, ⌜∀ (a:Addr), a ∈ (addr_of_page p) -> is_Some (mem !! a)⌝ ∗ [∗ map] a ↦ w ∈ mem, (a ->a w))%I.
 
   (** definition **)
 
@@ -30,61 +30,95 @@ Section logrel.
   Definition pgt_entries_own_excl (ps: gset PID) (vo: VMID) (be:bool) : iProp Σ:=
     [∗ set] p ∈ ps, p -@O> vo ∗ p -@E> be.
 
-  Definition tran_entries (trans: gmap Addr transaction) : iProp Σ:=
-    [∗ map] h ↦ tran ∈ trans , h ->t tran.1 ∗ h ->re tran.2 .
+  (* [transferred_tran_entries] includes all transaction related entries transferred to/from i from/to primary when scheduling,*)
+  Definition transferred_tran_entries (trans: gmap Addr transaction) : iProp Σ:=
+    [∗ map] h ↦ tran ∈ trans ,
+        (* All of half of transactions are required, as we don't know which one would be used by i.
+          Only *half* is needed so that related vms can remember transactions by keeping the other half. *)
+        h -{1/2}>t tran.1 ∗
+        (* If i is the sender or receiver of a donation, the other half of transaction entry is required.
+            Since it is possible for i to retrieve/reclaim the transaction, getting the whole entry removed.*)
+        (⌜(tran.1.1.1.1.1 = i ∨ tran.1.1.1.2 = i) ∧ tran.1.2 = Donation⌝ -∗ h -{1/2}>t tran.1) ∗
+        (* Retrievals must be provided so that i as the receiver is able to retrieve/relinquish. *)
+        (⌜tran.1.1.1.2 = i⌝ -∗ h ->re tran.2) ∗
+        (* Donation is again special here due to the same reason. *)
+        (⌜tran.1.1.1.1.1 = i ∧ tran.1.2 = Donation⌝ -∗ h ->re tran.2 ∗ ⌜tran.2 = false⌝).
 
-  Definition tran_carried_pgt_entries (trans :gmap Addr transaction): iProp Σ:=
-    [∗ map] h ↦ tran ∈ trans , if bool_decide ((tran.1.1.1.1.1 = i) ∨ (tran.1.2 = Donation)) then
-                                 ∃v b, pgt_entries_own_excl tran.1.1.2 v b
-                               else True.
+  (* [owned_trans_entries] are entries kept by i as the sender of non-donation transactions. *)
+  Definition owned_tran_entries (trans: gmap Addr transaction) : iProp Σ:=
+    [∗ map] h ↦ tran ∈ trans , ⌜tran.1.1.1.1.1 = i ∧ tran.1.2 ≠ Donation⌝ -∗ h -{1/2}>t tran.1.
 
-  Definition accessible_memory_cells (ps : gset PID) (mem:mem): iProp Σ :=
+  Definition transferred_pgt_entries (trans: gmap Addr transaction) : iProp Σ:=
+    [∗ map] h ↦ tran ∈ trans ,
+       ⌜(tran.1.1.1.1.1 = i ∧ tran.2 = true) ∨ (tran.1.1.1.2 = i ∧ tran.1.2 = Donation)⌝ -∗
+           pgt_entries_own_excl tran.1.1.2 tran.1.1.1.1.1 tran.2.
+
+  Definition memory_cells (ps : gset PID) : iProp Σ :=
     [∗ set] p ∈ ps, unknown_mem_page p.
 
-  Definition ps_trans (trans: gmap Addr transaction) : gset PID :=
-    map_fold (λ (k:Addr) (v:transaction) acc, v.1.1.2 ∪ acc) (∅: gset PID) trans.
+  (* TODO: alternative definition, many lemmas in [logrel_extra.v] need to be proved to use it *)
+  Definition memory_cell' (ps :gset PID): iProp Σ:=
+    ∃ mem, (⌜dom (gset Addr) mem = (set_fold (λ p acc, list_to_set (addr_of_page p) ∪ acc) ∅ ps)⌝ ∗ [∗ map] k ↦ v ∈ mem, k ->a v)%I.
 
-  Program Definition interp_access: iPropO Σ:=
-    (∃ regs,
+
+  Definition accessible_trans (trans : gmap Word transaction) :=
+   filter (λ kv, (kv.2.1.1.1.1.1 = i ∧ kv.2.1.2 = Sharing) ∨ (kv.2.1.1.1.2 = i ∧ kv.2.2 = true)) trans.
+
+  Definition ps_trans (trans: gmap Word transaction) : gset PID :=
+    map_fold (λ (k:Addr) v acc, v.1.1.2 ∪ acc) (∅: gset PID) trans.
+
+  Program Definition interp_access ps_acc p_tx p_rx (trans : gmap Word transaction) : iPropO Σ:=
+    (
+      let ps_nea := ps_trans (accessible_trans trans) ∪ {[p_rx]} in
+      let ps_ea := ps_acc ∖ ps_nea in
       (* registers *)
-      (⌜is_total_gmap regs⌝ ∗ [∗ map] r ↦ w ∈ regs, r @@ i ->r w) ∗
+      (∃ regs, ⌜is_total_gmap regs⌝ ∗ [∗ map] r ↦ w ∈ regs, r @@ i ->r w) ∗
       (* mailbox *)
-      (∃ p, RX@i := p) ∗ (∃ p, TX@i := p) ∗
+      (TX@i := p_tx) ∗
+      (* access *)
+      i -@A> [ps_acc] ∗
+      (* own & excl *)
+      pgt_entries_own_excl ps_ea i true ∗
+      (* transaction *)
+      owned_tran_entries trans ∗
+      ⌜ ps_nea ⊆ ps_acc ⌝ ∗
+      (* mem *)
+      memory_cells ps_ea ∗
       (* VMProp *)
-      VMProp i
-      ( (∃  mem ps_na ps_acc trans hpool,
-            let ps_trans := ps_trans (trans) in
-            let ps_oea := ps_acc ∖ ps_trans in
-        (* lower bound *)
-        LB@ i := [ps_na] ∗ ⌜ps_na ## ps_acc⌝ ∗
-        (* resources *)
-        i -@A> [ps_acc] ∗
-        hp [hpool] ∗ tran_entries trans ∗
-        pgt_entries_own_excl ps_oea i true ∗
-        tran_carried_pgt_entries trans ∗
-        accessible_memory_cells ps_acc mem ∗
-        R0 @@ V0 ->r encode_hvc_func(Run) ∗ R1 @@ V0 ->r encode_vmid(i)) ∗
-        (* if i yielding, we give following resources back to pvm *)
-        VMProp V0 (
-          ∃ mem ps_na ps_acc trans hpool,
-            let ps_trans := ps_trans (trans) in
-            let ps_oea := ps_acc ∖ ps_trans in
-          (* lower bound *)
-          LB@ i := [ps_na] ∗ ⌜ps_na ## ps_acc⌝ ∗
-          (* resources *)
-          i -@A> [ps_acc] ∗
-          hp [hpool] ∗ tran_entries trans ∗
-          pgt_entries_own_excl ps_oea i true ∗
-          tran_carried_pgt_entries trans ∗
-          accessible_memory_cells ps_acc mem ∗
-          (* R0 and R1 of pvm *)
-          (R0 @@ V0 ->r encode_hvc_func(Yield) ∗ R1 @@ V0 ->r encode_vmid(i))
-          (* no scheduling, we finish the proof *)
-          (* NOTE: if i will be scheduled arbitrary number of times, need recursive definition *)
-          ∨ False) (1/2)%Qp ∗
-        (* status of RX *)
-        (RX@ i :=() ∨ ∃ w s, RX@ i :=(w, s)))
-      (1/2)%Qp
+      VMProp i ((∃ ps_na (trans' : gmap Word transaction) hpool,
+                    let ps_trans' := ps_trans (accessible_trans trans') in
+                    ⌜accessible_trans trans = accessible_trans trans'⌝ ∗
+                    (* lower bound *)
+                    LB@ i := [ps_na] ∗ ⌜ps_na ## ps_acc⌝ ∗
+                    (* we need this to ensure all transaction entries are transferred *)
+                    ⌜inv_trans_hpool_consistent' trans' hpool⌝ ∗
+                    (* transaction entries *)
+                    hp [hpool] ∗ transferred_tran_entries trans' ∗
+                    (* page table entries *)
+                    transferred_pgt_entries trans' ∗
+                    (* mem *)
+                    memory_cells ps_trans' ∗
+                    (* status of RX *)
+                    (RX@ i :=() ∨ ∃l s, RX@i :=(l,s)) ∗
+                    (* RX *)
+                    (RX@i := p_rx ∗ memory_cells {[p_rx]})) ∗
+                  R0 @@ V0 ->r encode_hvc_func(Run) ∗ R1 @@ V0 ->r encode_vmid(i) ∗
+                  (* if i yielding, we give following resources back to pvm *)
+                  VMProp V0 (
+                           ∃ ps_na' ps_acc' trans'' hpool',
+                             let ps_trans'' := ps_trans (accessible_trans trans'') in
+                             (* lower bound *)
+                             LB@ i := [ps_na'] ∗ ⌜ps_na' ## ps_acc'⌝ ∗
+                                        (* resources *)
+                                        hp [hpool'] ∗ transferred_tran_entries trans'' ∗
+                                        transferred_pgt_entries trans'' ∗
+                                        memory_cells ps_trans'' ∗
+                                        (* R0 and R1 of pvm *)
+                                        (R0 @@ V0 ->r encode_hvc_func(Yield) ∗ R1 @@ V0 ->r encode_vmid(i))
+                                      (* no scheduling, we finish the proof *)
+                                      (* NOTE: if i will be scheduled arbitrary number of times, need recursive definition *)
+                                      ∨ False) (1/2)%Qp)
+               (1/2)%Qp
     )%I.
 
 End logrel.
