theories/logrel/fundamental.v
@@ -1,8 +1,8 @@
 From iris.proofmode Require Import tactics.
 From machine_program_logic.program_logic Require Import weakestpre.
 From HypVeri.lang Require Import lang.
-From HypVeri.algebra Require Import base.
-From HypVeri.rules Require Import rules_base nop mov ldr str halt fail add sub mult cmp.
+From HypVeri.algebra Require Import base pagetable.
+From HypVeri.rules Require Import rules_base nop mov (* ldr str halt fail add sub mult cmp *).
 From HypVeri.logrel Require Import logrel logrel_extra.
 From HypVeri Require Import proofmode.
 Import uPred.
@@ -12,586 +12,583 @@ Section fundamental.
   Context `{hypparams:!HypervisorParameters}.
   Context `{vmG: !gen_VMG Σ}.
 
-
   (* TODO:
-   - [x] fix iIntros
-   - [] fix pgt accessor
-   - [x] new lemmas for updating VMProp (not necessary)
-   - [x] fix nop
-   - [x] fix mov
-   - [x] str
-   - [x] ldr
-   - [x] merging excl and shared pgt
+   - [] new lemmas for updating VMProp (not necessary)
+   - [] str
    - [] fix mem_send_nz.v
    - [] mem share *)
 
   (* TODO: separate into helper lemmas *)
   Lemma ftlr (i:VMID)  :
-   ∀ pgt, interp_access i pgt ⊢ interp_execute i.
+  ∀ ps_acc p_tx p_rx trans, interp_access i ps_acc p_tx p_rx trans ⊢ interp_execute i.
   Proof.
     rewrite /interp_access /=.
-    iLöb as "IH".
-    iIntros (pgt) "(%regs & (#Htotal_regs & regs) & rx & tx & VMProp) Hnotp VMProp_holds".
-    iDestruct (VMProp_holds_agree i with "[$VMProp_holds $VMProp]") as "[Hres VMProp]".
-    (* iEval (rewrite later_or) in "Hres". *)
-    (* iDestruct "Hres" as "[Hres| >False]";last done. *)
-    iDestruct( later_exist with "Hres") as (mem) "Hres".
-    iDestruct( later_exist with "Hres") as (shandle) "Hres".
-    (* the vm is scheduled *)
-    rewrite !later_sep.
-    (* we have to do this because VMProp is not(?) timeless *)
-    iDestruct "Hres" as "(>#Htotal_pgt & >Hhpool & >#Htotal_mem & >R0z & >R1z & (VMPropz & >pgt & >mem & >rx_status))".
+    (* iLöb as "IH". *)
+    iIntros (ps_acc p_tx p_rx trans) "((%regs & #Htotal_regs & regs) & tx & pgt_acc & pgt_owned & trans_owned & #Hps_incl & mem_owned & VMProp) Hnotp VMProp_holds".
+    iDestruct (VMProp_holds_agree i with "[$VMProp_holds $VMProp]") as "[Hres _]".
+    iEval (rewrite later_sep) in "Hres".
+    iDestruct "Hres" as "[>Hres1 Hres]".
+    iLöb as "IH" forall (regs ps_acc trans) "Htotal_regs Hps_incl".
     (* we don't really need to get the resource of PC, but just the value *)
-    iPoseProof ("Htotal_regs" $! PC) as "%Hlookup_PC".
+    iDestruct "Hres1" as (ps_na trans' hpool) "(%Heq_acc_trans & LB & %Hdisj_ps & %Hinv_trans & hp & trans_transferred &
+                         pgt_transferred & mem_transferred & rx_state & rx & mem_rx)".
+    iDestruct "Hps_incl" as %Hps_incl.
+    iAssert (memory_cells ps_acc)%I with "[mem_owned mem_transferred mem_rx]" as "mem".
+    {
+      iDestruct (memory_cells_disj with "[$mem_rx $mem_transferred]") as %Hdisj_ps_rx.
+      rewrite /memory_cells.
+      rewrite Heq_acc_trans.
+      assert (ps_acc = (ps_acc ∖ (ps_trans (accessible_trans i trans') ∪ {[p_rx]})) ∪ (ps_trans (accessible_trans i trans') ∪ {[p_rx]})) as Hps_eq.
+      {
+        rewrite -Heq_acc_trans.
+        rewrite difference_union_L.
+        rewrite union_comm_L.
+        rewrite subseteq_union_1_L //.
+      }
+      iEval (rewrite Hps_eq).
+      rewrite big_opS_union;last set_solver +.
+      iFrame "mem_owned".
+      rewrite big_opS_union; last set_solver + Hdisj_ps_rx.
+      iFrame.
+    }
+
+    iDestruct "Htotal_regs" as %Htotal_regs.
+    pose proof (Htotal_regs PC) as Hlookup_PC.
     destruct Hlookup_PC as [ai Hlookup_PC].
-    (* getting sacc from pgt *)
-    iPoseProof ("Htotal_pgt" $! (to_pid_aligned ai)) as "%Hlookup_ai".
-    destruct Hlookup_ai as [[? sacc] Hlookup_ai].
     (* sswp *)
     rewrite ->wp_sswp.
-    destruct (decide (i ∈ sacc)).
+    destruct (decide ((tpa ai) ∈ ps_acc)).
     { (* i has access *)
-      iEval(rewrite /pagetable) in "pgt".
-      iPoseProof ("Htotal_mem" $! ai) as "[%instr %Hlookup_instr]".
+      (* TODO: (tpa ai) ≠ tx *)
+      iEval (rewrite /memory_cells ) in "mem".
+      rewrite (big_sepS_delete _ ps_acc (tpa ai));last done.
+      iDestruct "mem" as "[[%mem_g (%His_some_mem_g & mem_pi)] mem]".
+      pose proof (His_some_mem_g ai) as His_some_mem_ai.
+      feed specialize His_some_mem_ai;first apply tpa_addr_of_page.
+      destruct His_some_mem_ai as [instr Hlookup_mem_ai].
       destruct (decode_instruction instr) as [instr'|] eqn:Heqn.
       { (* valid instruction *)
         destruct instr'.
         { (* nop *)
           (* getting the PC *)
-          iDestruct (reg_big_sepM_split_upd regs i Hlookup_PC with "[$Htotal_regs $regs]")
-            as "[PC Hacc_regs]".
-          (* getting pgt *)
-          (* we don't update pagetable *)
-          iDestruct (pgt_big_sepM_split pgt Hlookup_ai with "[$pgt]")
-            as "[[_ pi] Hacc_pgt]".
-          iDestruct ("pi" with "[]") as (q) "[pi p_instr_q]"; first done.
+          iDestruct (reg_big_sepM_split_upd regs i Hlookup_PC with "[$regs]")
+            as "[PC Hacc_regs]";first done.
           (* getting mem *)
-          rewrite /accessible_memory.
-          (* we don't update memory *)
-          iDestruct (mem_big_sepM_split mem Hlookup_instr with "[$mem]")
-            as "[instrm Hacc_mem]".
-          iDestruct ("instrm" with "[]") as "instrm".
-          { iPureIntro. exists (v,sacc).  split;done. }
-          iApply (nop ai (w1 := instr) with "[PC pi instrm]"); iFrameAutoSolve.
+          iDestruct (mem_big_sepM_split mem_g Hlookup_mem_ai with "[$mem_pi]")
+            as "[mem_instr mem_pi]".
+          iApply (nop ai (w1 := instr) with "[PC pgt_acc mem_instr]"); iFrameAutoSolve.
           iNext.
-          iIntros "(PC & instrm & pi) _".
+          iIntros "(PC & mem_instr & pgt_acc) _".
           iDestruct ("Hacc_regs" $! (ai ^+ 1)%f with "PC") as "[#Htotal_regs' regs]".
-          iDestruct ("Hacc_mem" with "[instrm]") as "mem".
-          { iIntros "_". iFrame "instrm". }
-          iDestruct ("Hacc_pgt" with "[pi p_instr_q]") as "pgt".
-          { iSplitL "". iIntros "%".  rewrite /= //in H. iIntros "_". iExists q. iFrame "pi p_instr_q". }
-          (* NOTE: accessor doesn't work on pagetable, since we could update it. need to extend interp_access *)
-          iDestruct (VMProp_split with "VMProp") as "[VMProp1 VMProp2]".
-          iSpecialize ("IH" $! pgt with "[regs $rx $tx VMProp1]").
-          iExists (<[PC:= (ai ^+ 1)%f]> regs).
-          iFrame.
-          iFrame "Htotal_regs'".
-          iSpecialize ("IH" with "Hnotp").
+          iDestruct ("mem_pi" with "[mem_instr]") as "mem_pi";  first iFrame.
+          (*TODO :split mem*)
+          iSpecialize ("IH" $! _ with "regs tx pgt_acc pgt_owned trans_owned [mem_pi mem] Hnotp
+                             [LB hp trans_transferred pgt_transferred $rx_state $rx] [$Hres]").
+          { admit. }
+          { iExists ps_na, trans', hpool. iFrame. admit. }
           iApply "IH".
-          set Pred := (X in VMProp i X _).
-          iExists Pred.
-          iFrame.
-          iNext.
-          iExists mem, shandle.
-          iFrame.
-          iFrame "#".
+          done.
+          done.
         }
         { (* mov *)
-          destruct src as [imm | srcreg].
-          { (* mov imm *)
-            destruct dst.
-            {
-              apply decode_instruction_valid in Heqn.
-              inversion Heqn.
-              unfold reg_valid_cond in *.
-              exfalso.
-              naive_solver.
-            }
-            {
-              apply decode_instruction_valid in Heqn.
-              inversion Heqn.
-              unfold reg_valid_cond in *.
-              exfalso.
-              naive_solver.
-            }
-            {
-              iPoseProof ("Htotal_regs" $! (R n fin)) as (w) "%Hlookup_R".
-              (* getting regs *)
-              iDestruct ((reg_big_sepM_split_upd2 regs i _ Hlookup_PC Hlookup_R)
-                          with "[$Htotal_regs $regs]") as "(PC & R & Hacc_regs)".
-              (* getting mem *)
-              rewrite /accessible_memory.
-              (* we don't update memory *)
-              iDestruct (mem_big_sepM_split mem Hlookup_instr with "[$mem]")
-                as "[instrm Hacc_mem]".
-              iDestruct ("instrm" with "[]") as "instrm".
-              { iPureIntro. exists (v,sacc).  split;done. }
-              (* getting pgt *)
-              (* we don't update pagetable *)
-              iDestruct (pgt_big_sepM_split pgt Hlookup_ai with "[$pgt]")
-                as "[[_ pi] Hacc_pgt]".
-              iDestruct ("pi" with "[]") as (q) "[pi p_instr_q]"; first done.
-              iApply (mov_word (w3 := w) _ imm (R n fin) with "[PC pi instrm R]"); iFrameAutoSolve.
-              iNext.
-              iIntros "(PC & instrm & pi & R) _".
-              iDestruct ("Hacc_regs" with "[$PC $R]") as (regs') "[#Htotal_regs' regs]";iFrame.
-              iDestruct ("Hacc_mem" with "[instrm]") as "mem".
-              { iIntros "_". iFrame "instrm". }
-              iDestruct ("Hacc_pgt" with "[pi p_instr_q]") as "pgt".
-              { iSplitL "". iIntros "%".  rewrite /= //in H. iIntros "_". iExists q. iFrame "pi p_instr_q". }
-              iDestruct (VMProp_split with "VMProp") as "[VMProp1 VMProp2]".
-              iSpecialize ("IH" $! pgt with "[regs Htotal_regs' rx tx VMProp1]").
-              iExists regs'.
-              iFrame.
-              iFrame "#".
-              iSpecialize ("IH" with "Hnotp").
-              iApply "IH".
-              set Pred := (X in VMProp i X _).
-              iExists Pred.
-              iFrame.
-              iNext.
-              iLeft.
-              iExists mem, shandle.
-              iFrame.
-              iFrame "#".
-            }
-          }
-          { (* mov reg *)
-            destruct dst.
-            {
-              apply decode_instruction_valid in Heqn.
-              inversion Heqn.
-              unfold reg_valid_cond in *.
-              exfalso.
-              naive_solver.
-            }
-            {
-              apply decode_instruction_valid in Heqn.
-              inversion Heqn.
-              unfold reg_valid_cond in *.
-              exfalso.
-              naive_solver.
-            }
-            destruct srcreg.
-            {
-              apply decode_instruction_valid in Heqn.
-              inversion Heqn.
-              unfold reg_valid_cond in *.
-              exfalso.
-              naive_solver.
-            }
-            {
-              apply decode_instruction_valid in Heqn.
-              inversion Heqn.
-              unfold reg_valid_cond in *.
-              exfalso.
-              naive_solver.
-            }
-            {
-              iPoseProof ("Htotal_regs" $! (R n fin)) as (w) "%Hlookup_R".
-              iPoseProof ("Htotal_regs" $! (R n0 fin0)) as (w') "%Hlookup_R'".
-              (* getting regs *)
-              
-              iDestruct ((reg_big_sepM_split_upd3 regs i _ _ _ Hlookup_PC Hlookup_R Hlookup_R')
-                          with "[$Htotal_regs $regs]") as "(PC & R & R' & Hacc_regs)".
-              (* getting mem *)
-              rewrite /accessible_memory.
-              (* we don't update memory *)
-              iDestruct (mem_big_sepM_split mem Hlookup_instr with "[$mem]")
-                as "[instrm Hacc_mem]".
-              iDestruct ("instrm" with "[]") as "instrm".
-              { iPureIntro. exists (v,sacc).  split;done. }
-              (* getting pgt *)
-              (* we don't update pagetable *)
-              iDestruct (pgt_big_sepM_split pgt Hlookup_ai with "[$pgt]")
-                as "[[_ pi] Hacc_pgt]".
-              iDestruct ("pi" with "[]") as (q) "[pi p_instr_q]"; first done.
-              iApply (mov_reg (w3 := w') _ _ (R n fin) (R n0 fin0) with "[PC pi instrm R R']"); iFrameAutoSolve.
-              iNext.
-              iIntros "(PC & instrm & pi & R & R') _".
-              iDestruct ("Hacc_regs" with "[$PC $R $R']") as (regs') "[#Htotal_regs' regs]";iFrame.
-              iDestruct ("Hacc_mem" with "[instrm]") as "mem".
-              { iIntros "_". iFrame "instrm". }
-              iDestruct ("Hacc_pgt" with "[pi p_instr_q]") as "pgt".
-              { iSplitL "". iIntros "%".  rewrite /= //in H. iIntros "_". iExists q. iFrame "pi p_instr_q". }
-              iDestruct (VMProp_split with "VMProp") as "[VMProp1 VMProp2]".
-              iSpecialize ("IH" $! pgt with "[regs Htotal_regs' rx tx VMProp1]").
-              iExists regs'.
-              iFrame.
-              iFrame "#".
-              iSpecialize ("IH" with "Hnotp").
-              iApply "IH".
-              set Pred := (X in VMProp i X _).
-              iExists Pred.
-              iFrame.
-              iNext.
-              iLeft.
-              iExists mem, shandle.
-              iFrame.
-              iFrame "#".
-            }
-          }
+          admit.
+          (* destruct src as [imm | srcreg]. *)
+          (* { (* mov imm *) *)
+          (*   destruct dst. *)
+          (*   { *)
+          (*     apply decode_instruction_valid in Heqn. *)
+          (*     inversion Heqn. *)
+          (*     unfold reg_valid_cond in *. *)
+          (*     exfalso. *)
+          (*     naive_solver. *)
+          (*   } *)
+          (*   { *)
+          (*     apply decode_instruction_valid in Heqn. *)
+          (*     inversion Heqn. *)
+          (*     unfold reg_valid_cond in *. *)
+          (*     exfalso. *)
+          (*     naive_solver. *)
+          (*   } *)
+          (*   { *)
+          (*     iPoseProof ("Htotal_regs" $! (R n fin)) as (w) "%Hlookup_R". *)
+          (*     (* getting regs *) *)
+          (*     iDestruct ((reg_big_sepM_split_upd2 regs i _ Hlookup_PC Hlookup_R) *)
+          (*                 with "[$Htotal_regs $regs]") as "(PC & R & Hacc_regs)". *)
+          (*     (* getting mem *) *)
+          (*     rewrite /accessible_memory. *)
+          (*     (* we don't update memory *) *)
+          (*     iDestruct (mem_big_sepM_split mem Hlookup_instr with "[$mem]") *)
+          (*       as "[instrm Hacc_mem]". *)
+          (*     iDestruct ("instrm" with "[]") as "instrm". *)
+          (*     { iPureIntro. exists (v,sacc).  split;done. } *)
+          (*     (* getting pgt *) *)
+          (*     (* we don't update pagetable *) *)
+          (*     iDestruct (pgt_big_sepM_split pgt Hlookup_ai with "[$pgt]") *)
+          (*       as "[[_ pi] Hacc_pgt]". *)
+          (*     iDestruct ("pi" with "[]") as (q) "[pi p_instr_q]"; first done. *)
+          (*     iApply (mov_word (w3 := w) _ imm (R n fin) with "[PC pi instrm R]"); iFrameAutoSolve. *)
+          (*     iNext. *)
+          (*     iIntros "(PC & instrm & pi & R) _". *)
+          (*     iDestruct ("Hacc_regs" with "[$PC $R]") as (regs') "[#Htotal_regs' regs]";iFrame. *)
+          (*     iDestruct ("Hacc_mem" with "[instrm]") as "mem". *)
+          (*     { iIntros "_". iFrame "instrm". } *)
+          (*     iDestruct ("Hacc_pgt" with "[pi p_instr_q]") as "pgt". *)
+          (*     { iSplitL "". iIntros "%".  rewrite /= //in H. iIntros "_". iExists q. iFrame "pi p_instr_q". } *)
+          (*     iDestruct (VMProp_split with "VMProp") as "[VMProp1 VMProp2]". *)
+          (*     iSpecialize ("IH" $! pgt with "[regs Htotal_regs' rx tx VMProp1]"). *)
+          (*     iExists regs'. *)
+          (*     iFrame. *)
+          (*     iFrame "#". *)
+          (*     iSpecialize ("IH" with "Hnotp"). *)
+          (*     iApply "IH". *)
+          (*     set Pred := (X in VMProp i X _). *)
+          (*     iExists Pred. *)
+          (*     iFrame. *)
+          (*     iNext. *)
+          (*     iLeft. *)
+          (*     iExists mem, shandle. *)
+          (*     iFrame. *)
+          (*     iFrame "#". *)
+          (*   } *)
+          (* } *)
+          (* { (* mov reg *) *)
+          (*   destruct dst. *)
+          (*   { *)
+          (*     apply decode_instruction_valid in Heqn. *)
+          (*     inversion Heqn. *)
+          (*     unfold reg_valid_cond in *. *)
+          (*     exfalso. *)
+          (*     naive_solver. *)
+          (*   } *)
+          (*   { *)
+          (*     apply decode_instruction_valid in Heqn. *)
+          (*     inversion Heqn. *)
+          (*     unfold reg_valid_cond in *. *)
+          (*     exfalso. *)
+          (*     naive_solver. *)
+          (*   } *)
+          (*   destruct srcreg. *)
+          (*   { *)
+          (*     apply decode_instruction_valid in Heqn. *)
+          (*     inversion Heqn. *)
+          (*     unfold reg_valid_cond in *. *)
+          (*     exfalso. *)
+          (*     naive_solver. *)
+          (*   } *)
+          (*   { *)
+          (*     apply decode_instruction_valid in Heqn. *)
+          (*     inversion Heqn. *)
+          (*     unfold reg_valid_cond in *. *)
+          (*     exfalso. *)
+          (*     naive_solver. *)
+          (*   } *)
+          (*   { *)
+          (*     iPoseProof ("Htotal_regs" $! (R n fin)) as (w) "%Hlookup_R". *)
+          (*     iPoseProof ("Htotal_regs" $! (R n0 fin0)) as (w') "%Hlookup_R'". *)
+          (*     (* getting regs *) *)
+
+          (*     iDestruct ((reg_big_sepM_split_upd3 regs i _ _ _ Hlookup_PC Hlookup_R Hlookup_R') *)
+          (*                 with "[$Htotal_regs $regs]") as "(PC & R & R' & Hacc_regs)". *)
+          (*     (* getting mem *) *)
+          (*     rewrite /accessible_memory. *)
+          (*     (* we don't update memory *) *)
+          (*     iDestruct (mem_big_sepM_split mem Hlookup_instr with "[$mem]") *)
+          (*       as "[instrm Hacc_mem]". *)
+          (*     iDestruct ("instrm" with "[]") as "instrm". *)
+          (*     { iPureIntro. exists (v,sacc).  split;done. } *)
+          (*     (* getting pgt *) *)
+          (*     (* we don't update pagetable *) *)
+          (*     iDestruct (pgt_big_sepM_split pgt Hlookup_ai with "[$pgt]") *)
+          (*       as "[[_ pi] Hacc_pgt]". *)
+          (*     iDestruct ("pi" with "[]") as (q) "[pi p_instr_q]"; first done. *)
+          (*     iApply (mov_reg (w3 := w') _ _ (R n fin) (R n0 fin0) with "[PC pi instrm R R']"); iFrameAutoSolve. *)
+          (*     iNext. *)
+          (*     iIntros "(PC & instrm & pi & R & R') _". *)
+          (*     iDestruct ("Hacc_regs" with "[$PC $R $R']") as (regs') "[#Htotal_regs' regs]";iFrame. *)
+          (*     iDestruct ("Hacc_mem" with "[instrm]") as "mem". *)
+          (*     { iIntros "_". iFrame "instrm". } *)
+          (*     iDestruct ("Hacc_pgt" with "[pi p_instr_q]") as "pgt". *)
+          (*     { iSplitL "". iIntros "%".  rewrite /= //in H. iIntros "_". iExists q. iFrame "pi p_instr_q". } *)
+          (*     iDestruct (VMProp_split with "VMProp") as "[VMProp1 VMProp2]". *)
+          (*     iSpecialize ("IH" $! pgt with "[regs Htotal_regs' rx tx VMProp1]"). *)
+          (*     iExists regs'. *)
+          (*     iFrame. *)
+          (*     iFrame "#". *)
+          (*     iSpecialize ("IH" with "Hnotp"). *)
+          (*     iApply "IH". *)
+          (*     set Pred := (X in VMProp i X _). *)
+          (*     iExists Pred. *)
+          (*     iFrame. *)
+          (*     iNext. *)
+          (*     iLeft. *)
+          (*     iExists mem, shandle. *)
+          (*     iFrame. *)
+          (*     iFrame "#". *)
+          (*   } *)
+          (* } *)
         }
         { (* ldr *)
-          pose proof Heqn as Hdecode.
-          apply decode_instruction_valid in Heqn.
-          inversion Heqn as [| | ? ? Hvalid_dst Hvalid_src Hvalid_neq | | | | | | | | | ].
-          subst dst0 src0.
-          unfold reg_valid_cond in Hvalid_dst, Hvalid_src.
-          iPoseProof ("Htotal_regs" $! src) as (a_src) "%Hlookup_src".
-          iPoseProof ("Htotal_regs" $! dst) as (w_dst) "%Hlookup_dst".
-          iPoseProof ("Htotal_pgt" $! (tpa a_src)) as (perm_src) "%Hlookup_p_src".
-          iDestruct "tx" as (p_tx) "tx".
-          (* getting registers *)
-          iDestruct ((reg_big_sepM_split_upd3 regs i _ _ _ Hlookup_PC Hlookup_src Hlookup_dst)
-                      with "[$Htotal_regs $regs]") as "(PC & r_src & r_dst & Hacc_regs)".
-          (* case analysis on src  *)
-          destruct (decide (i ∈ perm_src.2)).
-          { (* has access to the page, more cases.. *)
-            destruct (decide((tpa a_src) = p_tx)).
-            { (* trying to read from tx page, fail *)
-              (* getting mem *)
-              rewrite /accessible_memory.
-              iDestruct (mem_big_sepM_split mem Hlookup_instr with "[$mem]")
-                as "[instrm Hacc_mem]".
-              iDestruct ("instrm" with "[]") as "a_instr".
-              { iPureIntro. exists (v,sacc).  split;done. }
-              (* getting pgt *)
-              iDestruct (pgt_big_sepM_split pgt Hlookup_ai with "[$pgt]")
-                as "[[_ pi] Hacc_pgt]".
-              iDestruct ("pi" with "[]") as (q) "[p_instr p_instr_q]"; first done.
-              iApply (ldr_access_tx ai a_src dst src with "[PC p_instr a_instr r_src r_dst tx]"); iFrameAutoSolve.
-              iNext.
-              iIntros "(tx & PC & a_instr & r_src & r_dst) _".
-              by iApply wp_terminated.
-            }
-            { (* normal case *)
-              destruct (decide ( a_src =ai)).
-              { (* exact same addr *)
-                iDestruct (pgt_big_sepM_split pgt Hlookup_ai with "[$pgt]")
-                  as "[[_ pi] Hacc_pgt]".
-                iDestruct ("pi" with "[]") as (q) "[p_instr p_instr_q]"; first done.
-                iDestruct (mem_big_sepM_split mem Hlookup_instr with "[$mem]")
-                  as "[instrm Hacc_mem]".
-                iDestruct ("instrm" with "[]") as "a_instr".
-                { iPureIntro. exists (v,sacc).  split;done. }
-                iApply (ldr_same_addr ai a_src dst src with "[PC p_instr a_instr r_src r_dst tx]"); iFrameAutoSolve.
-                { symmetry;done. }
-                iNext.
-                iIntros "(PC & a_instr & r_src & r_dst & p_instr & tx) _".
-                iDestruct ("Hacc_regs" with "[$PC $r_src $r_dst]") as (regs') "[#Htotal_regs' regs]";iFrame.
-                iDestruct ("Hacc_mem" with "[a_instr]") as "mem".
-                { iIntros "_". iFrame "a_instr". }
-                iDestruct ("Hacc_pgt" with "[p_instr p_instr_q]") as "pgt".
-                { iSplitL "". iIntros "%".  rewrite /= //in H. iIntros "_". iExists q. iFrame "p_instr p_instr_q". }
-                iDestruct (VMProp_split with "VMProp") as "[VMProp1 VMProp2]".
-                iSpecialize ("IH" $! pgt with "[regs Htotal_regs' rx tx VMProp1]").
-                iExists regs'.
-                iFrame.
-                iFrame "#".
-                iExists p_tx.
-                iFrame.
-                iSpecialize ("IH" with "Hnotp").
-                iApply "IH".
-                set Pred := (X in VMProp i X _).
-                iExists Pred.
-                iFrame.
-                iNext.
-                iLeft.
-                iExists mem, shandle.
-                iFrame.
-                iFrame "#".
-              }
-              { (* different addresses *)
-                iPoseProof ("Htotal_mem" $! a_src) as (w_src) "%Hlookup_a_src".
-                destruct (decide ((tpa a_src)=(tpa ai))).
-                { (* in same page *)
-                  iDestruct (pgt_big_sepM_split pgt Hlookup_ai with "[$pgt]")
-                    as "[[_ pi] Hacc_pgt]".
-                  iDestruct ("pi" with "[]") as (q) "[p_instr p_instr_q]"; first done.
-                  iDestruct (mem_big_sepM_split2 mem _ Hlookup_instr Hlookup_a_src with "[$mem]")
-                    as "[a_instr [a_src Hacc_mem]]".
-                  iDestruct ("a_instr" with "[]") as "a_instr".
-                  { iPureIntro. exists (v,sacc).  split;done. }
-                  iDestruct ("a_src" with "[]") as "a_src".
-                  { iPureIntro. exists (v,sacc).  split. rewrite e1 //. simpl;done. }
-                  iApply (ldr_same_page ai a_src dst src with "[PC p_instr a_instr a_src r_src r_dst tx]"); iFrameAutoSolve.
-                  { symmetry;done. }
-                  iNext.
-                  iIntros "(PC & a_instr & r_src & a_src & r_dst & p_instr & tx) _".
-                  iDestruct ("Hacc_regs" with "[$PC $r_src $r_dst]") as (regs') "[#Htotal_regs' regs]";iFrame.
-                  iDestruct ("Hacc_mem" with "[a_instr a_src]") as "mem".
-                  { iSplitL "a_instr".
-                    iIntros "_". iFrame "a_instr".
-                    iIntros "_". iFrame "a_src".
-                  }
-                  iDestruct ("Hacc_pgt" with "[p_instr p_instr_q]") as "pgt".
-                  { iSplitL "". iIntros "%".  rewrite /= //in H. iIntros "_". iExists q. iFrame "p_instr p_instr_q". }
-                  iDestruct (VMProp_split with "VMProp") as "[VMProp1 VMProp2]".
-                  iSpecialize ("IH" $! pgt with "[regs Htotal_regs' rx tx VMProp1]").
-                  iExists regs'.
-                  iFrame.
-                  iFrame "#".
-                  iExists p_tx.
-                  iFrame.
-                  iSpecialize ("IH" with "Hnotp").
-                  iApply "IH".
-                  set Pred := (X in VMProp i X _).
-                  iExists Pred.
-                  iFrame.
-                  iNext.
-                  iLeft.
-                  iExists mem, shandle.
-                  iFrame.
-                  iFrame "#".
-                }
-                { (* in difference pages *)
-                  iDestruct (pgt_big_sepM_split2 pgt _ Hlookup_ai Hlookup_p_src with "[$pgt]")
-                  as "([_ p_instr] & [_ p_src] & Hacc_pgt)".
-                  iDestruct ("p_instr" with "[]") as (q_i) "[p_instr p_instr_q]";first done.
-                  iDestruct ("p_src" with "[]") as (q_s) "[p_src p_src_q]";first done.
-                  (* getting mem *)
-                  rewrite /accessible_memory.
-                  iDestruct (mem_big_sepM_split2 mem _ Hlookup_instr Hlookup_a_src with "[$mem]")
-                    as "(a_instr & a_src & Hacc_mem)".
-                  iDestruct ("a_instr" with "[]") as "a_instr".
-                  { iPureIntro. exists (v,sacc).  split;done. }
-                  iDestruct ("a_src" with "[]") as "a_src".
-                  { iPureIntro. exists perm_src.  split;done. }
-                  iApply (ldr ai a_src dst src with "[PC p_instr p_src a_instr a_src r_src r_dst tx]"); iFrameAutoSolve.
-                  iNext.
-                  iIntros "(PC & a_instr & r_src & a_src & r_dst & p_instr & p_src & tx) _".
-                  iDestruct ("Hacc_regs" with "[$PC $r_src $r_dst]") as (regs') "[#Htotal_regs' regs]";iFrame.
-                  iDestruct ("Hacc_mem" with "[a_instr a_src]") as "mem".
-                  { iSplitL "a_instr".
-                    iIntros "_". iFrame "a_instr".
-                    iIntros "_". iFrame "a_src".
-                  }
-                  iDestruct ("Hacc_pgt" with "[p_instr p_src p_instr_q p_src_q]") as "pgt".
-                  { iSplitL "p_instr p_instr_q". iSplitL "". iIntros "%".  rewrite /= //in H. iIntros "_". iExists q_i. iFrame "p_instr p_instr_q".
-                    iSplitL "". iIntros "%".  rewrite /= //in H. iIntros "_". iExists q_s. iFrame "p_src p_src_q". }
-                  iDestruct (VMProp_split with "VMProp") as "[VMProp1 VMProp2]".
-                  iSpecialize ("IH" $! pgt with "[regs Htotal_regs' rx tx VMProp1]").
-                  iExists regs'.
-                  iFrame.
-                  iFrame "#".
-                  iExists p_tx.
-                  iFrame.
-                  iSpecialize ("IH" with "Hnotp").
-                  iApply "IH".
-                  set Pred := (X in VMProp i X _).
-                  iExists Pred.
-                  iFrame.
-                  iNext.
-                  iLeft.
-                  iExists mem, shandle.
-                  iFrame.
-                  iFrame "#".
-                }
-              }
-            }
-          }
-          { (* no access to the page, apply ldr_error *)
-            (* getting mem *)
-            rewrite /accessible_memory.
-            (* we don't update memory *)
-            iDestruct (mem_big_sepM_split mem Hlookup_instr with "[$mem]")
-              as "[instrm Hacc_mem]".
-            iDestruct ("instrm" with "[]") as "a_instr".
-            { iPureIntro. exists (v,sacc).  split;done. }
-            (* getting pgt *)
-            (* we don't update pagetable *)
-            iDestruct (pgt_big_sepM_split2 pgt _ Hlookup_ai Hlookup_p_src with "[$pgt]")
-              as "([_ p_instr] & [p_src _] & Hacc_pgt)".
-            iDestruct ("p_instr" with "[]") as (q_i) "[p_instr p_instr_q]";first done.
-            iDestruct ("p_src" with "[]") as "p_src";first done.
-            iApply (ldr_no_access ai a_src dst src with "[PC p_instr a_instr r_src r_dst tx p_src]"); iFrameAutoSolve.
-            iNext.
-            iIntros "(tx & PC & a_instr & r_src & p_src & r_dst) _".
-            by iApply wp_terminated.
-          }
+          admit.
+          (* pose proof Heqn as Hdecode. *)
+          (* apply decode_instruction_valid in Heqn. *)
+          (* inversion Heqn as [| | ? ? Hvalid_dst Hvalid_src Hvalid_neq | | | | | | | | | ]. *)
+          (* subst dst0 src0. *)
+          (* unfold reg_valid_cond in Hvalid_dst, Hvalid_src. *)
+          (* iPoseProof ("Htotal_regs" $! src) as (a_src) "%Hlookup_src". *)
+          (* iPoseProof ("Htotal_regs" $! dst) as (w_dst) "%Hlookup_dst". *)
+          (* iPoseProof ("Htotal_pgt" $! (tpa a_src)) as (perm_src) "%Hlookup_p_src". *)
+          (* iDestruct "tx" as (p_tx) "tx". *)
+          (* (* getting registers *) *)
+          (* iDestruct ((reg_big_sepM_split_upd3 regs i _ _ _ Hlookup_PC Hlookup_src Hlookup_dst) *)
+          (*             with "[$Htotal_regs $regs]") as "(PC & r_src & r_dst & Hacc_regs)". *)
+          (* (* case analysis on src  *) *)
+          (* destruct (decide (i ∈ perm_src.2)). *)
+          (* { (* has access to the page, more cases.. *) *)
+          (*   destruct (decide((tpa a_src) = p_tx)). *)
+          (*   { (* trying to read from tx page, fail *) *)
+          (*     (* getting mem *) *)
+          (*     rewrite /accessible_memory. *)
+          (*     iDestruct (mem_big_sepM_split mem Hlookup_instr with "[$mem]") *)
+          (*       as "[instrm Hacc_mem]". *)
+          (*     iDestruct ("instrm" with "[]") as "a_instr". *)
+          (*     { iPureIntro. exists (v,sacc).  split;done. } *)
+          (*     (* getting pgt *) *)
+          (*     iDestruct (pgt_big_sepM_split pgt Hlookup_ai with "[$pgt]") *)
+          (*       as "[[_ pi] Hacc_pgt]". *)
+          (*     iDestruct ("pi" with "[]") as (q) "[p_instr p_instr_q]"; first done. *)
+          (*     iApply (ldr_access_tx ai a_src dst src with "[PC p_instr a_instr r_src r_dst tx]"); iFrameAutoSolve. *)
+          (*     iNext. *)
+          (*     iIntros "(tx & PC & a_instr & r_src & r_dst) _". *)
+          (*     by iApply wp_terminated. *)
+          (*   } *)
+          (*   { (* normal case *) *)
+          (*     destruct (decide ( a_src =ai)). *)
+          (*     { (* exact same addr *) *)
+          (*       iDestruct (pgt_big_sepM_split pgt Hlookup_ai with "[$pgt]") *)
+          (*         as "[[_ pi] Hacc_pgt]". *)
+          (*       iDestruct ("pi" with "[]") as (q) "[p_instr p_instr_q]"; first done. *)
+          (*       iDestruct (mem_big_sepM_split mem Hlookup_instr with "[$mem]") *)
+          (*         as "[instrm Hacc_mem]". *)
+          (*       iDestruct ("instrm" with "[]") as "a_instr". *)
+          (*       { iPureIntro. exists (v,sacc).  split;done. } *)
+          (*       iApply (ldr_same_addr ai a_src dst src with "[PC p_instr a_instr r_src r_dst tx]"); iFrameAutoSolve. *)
+          (*       { symmetry;done. } *)
+          (*       iNext. *)
+          (*       iIntros "(PC & a_instr & r_src & r_dst & p_instr & tx) _". *)
+          (*       iDestruct ("Hacc_regs" with "[$PC $r_src $r_dst]") as (regs') "[#Htotal_regs' regs]";iFrame. *)
+          (*       iDestruct ("Hacc_mem" with "[a_instr]") as "mem". *)
+          (*       { iIntros "_". iFrame "a_instr". } *)
+          (*       iDestruct ("Hacc_pgt" with "[p_instr p_instr_q]") as "pgt". *)
+          (*       { iSplitL "". iIntros "%".  rewrite /= //in H. iIntros "_". iExists q. iFrame "p_instr p_instr_q". } *)
+          (*       iDestruct (VMProp_split with "VMProp") as "[VMProp1 VMProp2]". *)
+          (*       iSpecialize ("IH" $! pgt with "[regs Htotal_regs' rx tx VMProp1]"). *)
+          (*       iExists regs'. *)
+          (*       iFrame. *)
+          (*       iFrame "#". *)
+          (*       iExists p_tx. *)
+          (*       iFrame. *)
+          (*       iSpecialize ("IH" with "Hnotp"). *)
+          (*       iApply "IH". *)
+          (*       set Pred := (X in VMProp i X _). *)
+          (*       iExists Pred. *)
+          (*       iFrame. *)
+          (*       iNext. *)
+          (*       iLeft. *)
+          (*       iExists mem, shandle. *)
+          (*       iFrame. *)
+          (*       iFrame "#". *)
+          (*     } *)
+          (*     { (* different addresses *) *)
+          (*       iPoseProof ("Htotal_mem" $! a_src) as (w_src) "%Hlookup_a_src". *)
+          (*       destruct (decide ((tpa a_src)=(tpa ai))). *)
+          (*       { (* in same page *) *)
+          (*         iDestruct (pgt_big_sepM_split pgt Hlookup_ai with "[$pgt]") *)
+          (*           as "[[_ pi] Hacc_pgt]". *)
+          (*         iDestruct ("pi" with "[]") as (q) "[p_instr p_instr_q]"; first done. *)
+          (*         iDestruct (mem_big_sepM_split2 mem _ Hlookup_instr Hlookup_a_src with "[$mem]") *)
+          (*           as "[a_instr [a_src Hacc_mem]]". *)
+          (*         iDestruct ("a_instr" with "[]") as "a_instr". *)
+          (*         { iPureIntro. exists (v,sacc).  split;done. } *)
+          (*         iDestruct ("a_src" with "[]") as "a_src". *)
+          (*         { iPureIntro. exists (v,sacc).  split. rewrite e1 //. simpl;done. } *)
+          (*         iApply (ldr_same_page ai a_src dst src with "[PC p_instr a_instr a_src r_src r_dst tx]"); iFrameAutoSolve. *)
+          (*         { symmetry;done. } *)
+          (*         iNext. *)
+          (*         iIntros "(PC & a_instr & r_src & a_src & r_dst & p_instr & tx) _". *)
+          (*         iDestruct ("Hacc_regs" with "[$PC $r_src $r_dst]") as (regs') "[#Htotal_regs' regs]";iFrame. *)
+          (*         iDestruct ("Hacc_mem" with "[a_instr a_src]") as "mem". *)
+          (*         { iSplitL "a_instr". *)
+          (*           iIntros "_". iFrame "a_instr". *)
+          (*           iIntros "_". iFrame "a_src". *)
+          (*         } *)
+          (*         iDestruct ("Hacc_pgt" with "[p_instr p_instr_q]") as "pgt". *)
+          (*         { iSplitL "". iIntros "%".  rewrite /= //in H. iIntros "_". iExists q. iFrame "p_instr p_instr_q". } *)
+          (*         iDestruct (VMProp_split with "VMProp") as "[VMProp1 VMProp2]". *)
+          (*         iSpecialize ("IH" $! pgt with "[regs Htotal_regs' rx tx VMProp1]"). *)
+          (*         iExists regs'. *)
+          (*         iFrame. *)
+          (*         iFrame "#". *)
+          (*         iExists p_tx. *)
+          (*         iFrame. *)
+          (*         iSpecialize ("IH" with "Hnotp"). *)
+          (*         iApply "IH". *)
+          (*         set Pred := (X in VMProp i X _). *)
+          (*         iExists Pred. *)
+          (*         iFrame. *)
+          (*         iNext. *)
+          (*         iLeft. *)
+          (*         iExists mem, shandle. *)
+          (*         iFrame. *)
+          (*         iFrame "#". *)
+          (*       } *)
+          (*       { (* in difference pages *) *)
+          (*         iDestruct (pgt_big_sepM_split2 pgt _ Hlookup_ai Hlookup_p_src with "[$pgt]") *)
+          (*         as "([_ p_instr] & [_ p_src] & Hacc_pgt)". *)
+          (*         iDestruct ("p_instr" with "[]") as (q_i) "[p_instr p_instr_q]";first done. *)
+          (*         iDestruct ("p_src" with "[]") as (q_s) "[p_src p_src_q]";first done. *)
+          (*         (* getting mem *) *)
+          (*         rewrite /accessible_memory. *)
+          (*         iDestruct (mem_big_sepM_split2 mem _ Hlookup_instr Hlookup_a_src with "[$mem]") *)
+          (*           as "(a_instr & a_src & Hacc_mem)". *)
+          (*         iDestruct ("a_instr" with "[]") as "a_instr". *)
+          (*         { iPureIntro. exists (v,sacc).  split;done. } *)
+          (*         iDestruct ("a_src" with "[]") as "a_src". *)
+          (*         { iPureIntro. exists perm_src.  split;done. } *)
+          (*         iApply (ldr ai a_src dst src with "[PC p_instr p_src a_instr a_src r_src r_dst tx]"); iFrameAutoSolve. *)
+          (*         iNext. *)
+          (*         iIntros "(PC & a_instr & r_src & a_src & r_dst & p_instr & p_src & tx) _". *)
+          (*         iDestruct ("Hacc_regs" with "[$PC $r_src $r_dst]") as (regs') "[#Htotal_regs' regs]";iFrame. *)
+          (*         iDestruct ("Hacc_mem" with "[a_instr a_src]") as "mem". *)
+          (*         { iSplitL "a_instr". *)
+          (*           iIntros "_". iFrame "a_instr". *)
+          (*           iIntros "_". iFrame "a_src". *)
+          (*         } *)
+          (*         iDestruct ("Hacc_pgt" with "[p_instr p_src p_instr_q p_src_q]") as "pgt". *)
+          (*         { iSplitL "p_instr p_instr_q". iSplitL "". iIntros "%".  rewrite /= //in H. iIntros "_". iExists q_i. iFrame "p_instr p_instr_q". *)
+          (*           iSplitL "". iIntros "%".  rewrite /= //in H. iIntros "_". iExists q_s. iFrame "p_src p_src_q". } *)
+          (*         iDestruct (VMProp_split with "VMProp") as "[VMProp1 VMProp2]". *)
+          (*         iSpecialize ("IH" $! pgt with "[regs Htotal_regs' rx tx VMProp1]"). *)
+          (*         iExists regs'. *)
+          (*         iFrame. *)
+          (*         iFrame "#". *)
+          (*         iExists p_tx. *)
+          (*         iFrame. *)
+          (*         iSpecialize ("IH" with "Hnotp"). *)
+          (*         iApply "IH". *)
+          (*         set Pred := (X in VMProp i X _). *)
+          (*         iExists Pred. *)
+          (*         iFrame. *)
+          (*         iNext. *)
+          (*         iLeft. *)
+          (*         iExists mem, shandle. *)
+          (*         iFrame. *)
+          (*         iFrame "#". *)
+          (*       } *)
+          (*     } *)
+          (*   } *)
+          (* } *)
+          (* { (* no access to the page, apply ldr_error *) *)
+          (*   (* getting mem *) *)
+          (*   rewrite /accessible_memory. *)
+          (*   (* we don't update memory *) *)
+          (*   iDestruct (mem_big_sepM_split mem Hlookup_instr with "[$mem]") *)
+          (*     as "[instrm Hacc_mem]". *)
+          (*   iDestruct ("instrm" with "[]") as "a_instr". *)
+          (*   { iPureIntro. exists (v,sacc).  split;done. } *)
+          (*   (* getting pgt *) *)
+          (*   (* we don't update pagetable *) *)
+          (*   iDestruct (pgt_big_sepM_split2 pgt _ Hlookup_ai Hlookup_p_src with "[$pgt]") *)
+          (*     as "([_ p_instr] & [p_src _] & Hacc_pgt)". *)
+          (*   iDestruct ("p_instr" with "[]") as (q_i) "[p_instr p_instr_q]";first done. *)
+          (*   iDestruct ("p_src" with "[]") as "p_src";first done. *)
+          (*   iApply (ldr_no_access ai a_src dst src with "[PC p_instr a_instr r_src r_dst tx p_src]"); iFrameAutoSolve. *)
+          (*   iNext. *)
+          (*   iIntros "(tx & PC & a_instr & r_src & p_src & r_dst) _". *)
+          (*   by iApply wp_terminated. *)
+          (* } *)
         }
         { (* str *)
-          pose proof Heqn as Hdecode.
-          apply decode_instruction_valid in Heqn.
-          inversion Heqn as [| | | ? ? Hvalid_dst Hvalid_src Hvalid_neq | | | | | | | | ].
-          subst dst0 src0.
-          unfold reg_valid_cond in Hvalid_dst, Hvalid_src.
-          iPoseProof ("Htotal_regs" $! src) as (w_src) "%Hlookup_src".
-          iPoseProof ("Htotal_regs" $! dst) as (a_dst) "%Hlookup_dst".
-          iPoseProof ("Htotal_pgt" $! (tpa a_dst)) as (perm_dst) "%Hlookup_p_dst".
-          iDestruct "rx" as (p_rx) "rx".
-          (* getting registers *)
-          iDestruct ((reg_big_sepM_split_upd3 regs i _ _ _ Hlookup_PC Hlookup_src Hlookup_dst)
-                       with "[$Htotal_regs $regs]") as "(PC & r_src & r_dst & Hacc_regs)".
-          (* case analysis on src  *)
-          destruct (decide (i ∈ perm_dst.2)).
-          { (* has access to the page, more cases.. *)
-            destruct (decide((tpa a_dst) = p_rx)).
-            { (* trying to write to rx page, fail *)
-              (* getting mem *)
-              rewrite /accessible_memory.
-              iDestruct (mem_big_sepM_split mem Hlookup_instr with "[$mem]")
-                as "[a_instr Hacc_mem]".
-              iDestruct ("a_instr" with "[]") as "a_instr".
-              { iPureIntro. exists (v,sacc). split;done. }
-              (* getting pgt *)
-              iDestruct (pgt_big_sepM_split pgt Hlookup_ai with "[$pgt]")
-                  as "([_ p_instr] & Hacc_pgt)".
-              (* iDestruct (pgt_big_sepM_split2 pgt _ Hlookup_ai Hlookup_p_dst with "[$pgt]") *)
-              (*   as "([_ p_instr] & [_ p_src] & Hacc_pgt)". *)
-              iDestruct ("p_instr" with "[]") as (q_i) "[p_instr p_instr_q]";first done.
-              iApply (str_access_rx ai a_dst src dst with "[PC p_instr a_instr r_src r_dst rx]"); iFrameAutoSolve.
-              iNext.
-              iIntros "(rx & PC & a_instr & r_src & r_dst) _".
-              by iApply wp_terminated.
-            }
-            { (* normal case *)
-              destruct (decide (a_dst =ai)).
-              { (* exact same addr *)
-                iDestruct (pgt_big_sepM_split pgt Hlookup_ai with "[$pgt]")
-                  as "([_ p_instr] & Hacc_pgt)".
-                iDestruct ("p_instr" with "[]") as (q_i) "[p_instr p_instr_q]";first done.
-                iDestruct (mem_big_sepM_split_upd mem Hlookup_instr with "[$mem $Htotal_mem]")
-                  as "[instrm Hacc_mem]".
-                iDestruct ("instrm" with "[]") as "a_instr".
-                { iPureIntro. exists (v,sacc). split;done. }
-                iApply (str_same_addr ai a_dst src dst with "[PC p_instr a_instr r_src r_dst rx]"); iFrameAutoSolve.
-                { symmetry;done. }
-                iNext.
-                iIntros "(PC & a_instr & r_src & r_dst & p_instr & rx) _".
-                iDestruct ("Hacc_regs" with "[$PC $r_src $r_dst]") as (regs') "[#Htotal_regs' regs]";iFrame.
-                iDestruct ("Hacc_mem" with "[a_instr]") as "[#Htotal_mem' mem]".
-                { iIntros "_". iFrame "a_instr". }
-                iDestruct ("Hacc_pgt" with "[p_instr p_instr_q]") as "pgt".
-                { iSplitL "". iIntros "%".  rewrite /= //in H. iIntros "_". iExists q_i. iFrame "p_instr p_instr_q". }
-                iDestruct (VMProp_split with "VMProp") as "[VMProp1 VMProp2]".
-                iSpecialize ("IH" $! pgt with "[regs Htotal_regs' rx tx VMProp1]").
-                iExists regs'.
-                iFrame.
-                iFrame "#".
-                iExists p_rx.
-                iFrame.
-                iSpecialize ("IH" with "Hnotp").
-                iApply "IH".
-                set Pred := (X in VMProp i X _).
-                iExists Pred.
-                iFrame.
-                iNext.
-                iLeft.
-                iExists (<[ai:=w_src]>mem), shandle.
-                iFrame.
-                iFrame "#".
-              }
-              { (* different addresses *)
-                iPoseProof ("Htotal_mem" $! a_dst) as (w_dst) "%Hlookup_a_dst".
-                destruct (decide ((tpa a_dst)=(tpa ai))).
-                { (* in same page *)
-                  iDestruct (pgt_big_sepM_split pgt Hlookup_ai with "[$pgt]")
-                    as "([_ p_instr] & Hacc_pgt)".
-                  iDestruct ("p_instr" with "[]") as (q_i) "[p_instr p_instr_q]";first done.
-                  iDestruct (mem_big_sepM_split_upd2 mem _ Hlookup_instr Hlookup_a_dst with "[$mem $Htotal_mem]")
-                    as "[a_instr [a_src Hacc_mem]]".
-                  iDestruct ("a_instr" with "[]") as "a_instr".
-                  { iPureIntro. exists (v, sacc).  split;done. }
-                  iDestruct ("a_src" with "[]") as "a_src".
-                  { iPureIntro. exists (v,sacc).  split. rewrite e1 //. simpl;done. }
-                  iApply (str_same_page ai a_dst src dst with "[PC p_instr a_instr a_src r_src r_dst rx]"); iFrameAutoSolve.
-                  { symmetry;done. }
-                  iNext.
-                  iIntros "(PC & a_instr & r_src & a_src & r_dst & p_instr & rx) _".
-                  iDestruct ("Hacc_regs" with "[$PC $r_src $r_dst]") as (regs') "[#Htotal_regs' regs]";iFrame.
-                  iDestruct ("Hacc_mem" with "[a_instr a_src]") as (mem') "[#Htotal_mem' mem]".
-                  { iSplitL "a_instr".
-                    iIntros "_". iFrame "a_instr".
-                    iIntros "_". iFrame "a_src".
-                  }
-                  iDestruct ("Hacc_pgt" with "[p_instr p_instr_q]") as "pgt".
-                  { iSplitL "". iIntros "%".  rewrite /= //in H. iIntros "_". iExists q_i. iFrame "p_instr p_instr_q". }
-                  iDestruct (VMProp_split with "VMProp") as "[VMProp1 VMProp2]".
-                  iSpecialize ("IH" $! pgt with "[regs Htotal_regs' rx tx VMProp1]").
-                  iExists regs'.
-                  iFrame.
-                  iFrame "#".
-                  iExists p_rx.
-                  iFrame.
-                  iSpecialize ("IH" with "Hnotp").
-                  iApply "IH".
-                  set Pred := (X in VMProp i X _).
-                  iExists Pred.
-                  iFrame.
-                  iNext.
-                  iLeft.
-                  iExists mem', shandle.
-                  iFrame.
-                  iFrame "#".
-                }
-                { (* in different pages *)
-                  (* getting pgt *)
-                  iDestruct (pgt_big_sepM_split2 pgt _ Hlookup_ai Hlookup_p_dst with "[$pgt]")
-                    as "([_ p_instr] & [_ p_src] & Hacc_pgt)".
-                  iDestruct ("p_instr" with "[]") as (q_i) "[p_instr p_instr_q]";first done.
-                  iDestruct ("p_src" with "[]") as (q_s) "[p_src p_src_q]";first done.
-                  (* getting mem *)
-                  rewrite /accessible_memory.
-                  iDestruct (mem_big_sepM_split_upd2 mem _ Hlookup_instr Hlookup_a_dst with "[$mem $Htotal_mem]")
-                    as "(a_instr & a_src & Hacc_mem)".
-                  iDestruct ("a_instr" with "[]") as "a_instr".
-                  { iPureIntro. exists (v,sacc).  split;done. }
-                  iDestruct ("a_src" with "[]") as "a_src".
-                  { iPureIntro. exists perm_dst.  split;done. }
-                  iApply (str ai a_dst src dst with "[PC p_instr p_src a_instr a_src r_src r_dst rx]"); iFrameAutoSolve.
-                  iNext.
-                  iIntros "(PC & a_instr & r_src & a_dst & r_dst & p_instr & p_src & rx) _".
-                  iDestruct ("Hacc_regs" with "[$PC $r_src $r_dst]") as (regs') "[#Htotal_regs' regs]";iFrame.
-                  iDestruct ("Hacc_mem" with "[a_instr a_dst]") as (mem') "[#Htotal_mem' mem]".
-                  { iSplitL "a_instr".
-                    iIntros "_". iFrame "a_instr".
-                    iIntros "_". iFrame "a_dst".
-                  }
-                  iDestruct ("Hacc_pgt" with "[p_instr p_instr_q p_src p_src_q]") as "pgt".
-                  { iSplitL "p_instr p_instr_q". iSplitL "". iIntros "%".  rewrite /= //in H. iIntros "_". iExists q_i. iFrame "p_instr p_instr_q".
-                    iSplitL "". iIntros "%".  rewrite /= //in H. iIntros "_". iExists q_s. iFrame "p_src p_src_q". }
-                  iDestruct (VMProp_split with "VMProp") as "[VMProp1 VMProp2]".
-                  iSpecialize ("IH" $! pgt with "[regs Htotal_regs' rx tx VMProp1]").
-                  iExists regs'.
-                  iFrame.
-                  iFrame "#".
-                  iExists p_rx.
-                  iFrame.
-                  iSpecialize ("IH" with "Hnotp").
-                  iApply "IH".
-                  set Pred := (X in VMProp i X _).
-                  iExists Pred.
-                  iFrame.
-                  iNext.
-                  iLeft.
-                  iExists mem', shandle.
-                  iFrame.
-                  iFrame "#".
-                }
-              }
-            }
-          }
-          { (* no access to the page, apply ldr_error *)
-            (* getting mem *)
-            rewrite /accessible_memory.
-            (* we don't update memory *)
-            iDestruct (mem_big_sepM_split mem Hlookup_instr with "[$mem]")
-              as "[instrm Hacc_mem]".
-            iDestruct ("instrm" with "[]") as "a_instr".
-            { iPureIntro. exists (v,sacc).  split;done. }
-            (* getting pgt *)
-            (* we don't update pagetable *)
-            iDestruct (pgt_big_sepM_split2 pgt _ Hlookup_ai Hlookup_p_dst with "[$pgt]")
-              as "([_ p_instr] & [p_dst _] & Hacc_pgt)".
-            iDestruct ("p_instr" with "[]") as (q_i) "[p_instr p_instr_q]";first done.
-            iDestruct ("p_dst" with "[]") as "p_dst";first done.
-            iApply (str_no_access ai a_dst src dst with "[PC p_instr a_instr r_src r_dst p_dst]"); iFrameAutoSolve.
-            iNext.
-            iIntros "(PC & a_instr & r_src & p_src & r_dst) _".
-            by iApply wp_terminated.            
-          }
+          admit.
+          (* pose proof Heqn as Hdecode. *)
+          (* apply decode_instruction_valid in Heqn. *)
+          (* inversion Heqn as [| | | ? ? Hvalid_dst Hvalid_src Hvalid_neq | | | | | | | | ]. *)
+          (* subst dst0 src0. *)
+          (* unfold reg_valid_cond in Hvalid_dst, Hvalid_src. *)
+          (* iPoseProof ("Htotal_regs" $! src) as (w_src) "%Hlookup_src". *)
+          (* iPoseProof ("Htotal_regs" $! dst) as (a_dst) "%Hlookup_dst". *)
+          (* iPoseProof ("Htotal_pgt" $! (tpa a_dst)) as (perm_dst) "%Hlookup_p_dst". *)
+          (* iDestruct "rx" as (p_rx) "rx". *)
+          (* (* getting registers *) *)
+          (* iDestruct ((reg_big_sepM_split_upd3 regs i _ _ _ Hlookup_PC Hlookup_src Hlookup_dst) *)
+          (*              with "[$Htotal_regs $regs]") as "(PC & r_src & r_dst & Hacc_regs)". *)
+          (* (* case analysis on src  *) *)
+          (* destruct (decide (i ∈ perm_dst.2)). *)
+          (* { (* has access to the page, more cases.. *) *)
+          (*   destruct (decide((tpa a_dst) = p_rx)). *)
+          (*   { (* trying to write to rx page, fail *) *)
+          (*     (* getting mem *) *)
+          (*     rewrite /accessible_memory. *)
+          (*     iDestruct (mem_big_sepM_split mem Hlookup_instr with "[$mem]") *)
+          (*       as "[a_instr Hacc_mem]". *)
+          (*     iDestruct ("a_instr" with "[]") as "a_instr". *)
+          (*     { iPureIntro. exists (v,sacc). split;done. } *)
+          (*     (* getting pgt *) *)
+          (*     iDestruct (pgt_big_sepM_split pgt Hlookup_ai with "[$pgt]") *)
+          (*         as "([_ p_instr] & Hacc_pgt)". *)
+          (*     (* iDestruct (pgt_big_sepM_split2 pgt _ Hlookup_ai Hlookup_p_dst with "[$pgt]") *) *)
+          (*     (*   as "([_ p_instr] & [_ p_src] & Hacc_pgt)". *) *)
+          (*     iDestruct ("p_instr" with "[]") as (q_i) "[p_instr p_instr_q]";first done. *)
+          (*     iApply (str_access_rx ai a_dst src dst with "[PC p_instr a_instr r_src r_dst rx]"); iFrameAutoSolve. *)
+          (*     iNext. *)
+          (*     iIntros "(rx & PC & a_instr & r_src & r_dst) _". *)
+          (*     by iApply wp_terminated. *)
+          (*   } *)
+          (*   { (* normal case *) *)
+          (*     destruct (decide (a_dst =ai)). *)
+          (*     { (* exact same addr *) *)
+          (*       iDestruct (pgt_big_sepM_split pgt Hlookup_ai with "[$pgt]") *)
+          (*         as "([_ p_instr] & Hacc_pgt)". *)
+          (*       iDestruct ("p_instr" with "[]") as (q_i) "[p_instr p_instr_q]";first done. *)
+          (*       iDestruct (mem_big_sepM_split_upd mem Hlookup_instr with "[$mem $Htotal_mem]") *)
+          (*         as "[instrm Hacc_mem]". *)
+          (*       iDestruct ("instrm" with "[]") as "a_instr". *)
+          (*       { iPureIntro. exists (v,sacc). split;done. } *)
+          (*       iApply (str_same_addr ai a_dst src dst with "[PC p_instr a_instr r_src r_dst rx]"); iFrameAutoSolve. *)
+          (*       { symmetry;done. } *)
+          (*       iNext. *)
+          (*       iIntros "(PC & a_instr & r_src & r_dst & p_instr & rx) _". *)
+          (*       iDestruct ("Hacc_regs" with "[$PC $r_src $r_dst]") as (regs') "[#Htotal_regs' regs]";iFrame. *)
+          (*       iDestruct ("Hacc_mem" with "[a_instr]") as "[#Htotal_mem' mem]". *)
+          (*       { iIntros "_". iFrame "a_instr". } *)
+          (*       iDestruct ("Hacc_pgt" with "[p_instr p_instr_q]") as "pgt". *)
+          (*       { iSplitL "". iIntros "%".  rewrite /= //in H. iIntros "_". iExists q_i. iFrame "p_instr p_instr_q". } *)
+          (*       iDestruct (VMProp_split with "VMProp") as "[VMProp1 VMProp2]". *)
+          (*       iSpecialize ("IH" $! pgt with "[regs Htotal_regs' rx tx VMProp1]"). *)
+          (*       iExists regs'. *)
+          (*       iFrame. *)
+          (*       iFrame "#". *)
+          (*       iExists p_rx. *)
+          (*       iFrame. *)
+          (*       iSpecialize ("IH" with "Hnotp"). *)
+          (*       iApply "IH". *)
+          (*       set Pred := (X in VMProp i X _). *)
+          (*       iExists Pred. *)
+          (*       iFrame. *)
+          (*       iNext. *)
+          (*       iLeft. *)
+          (*       iExists (<[ai:=w_src]>mem), shandle. *)
+          (*       iFrame. *)
+          (*       iFrame "#". *)
+          (*     } *)
+          (*     { (* different addresses *) *)
+          (*       iPoseProof ("Htotal_mem" $! a_dst) as (w_dst) "%Hlookup_a_dst". *)
+          (*       destruct (decide ((tpa a_dst)=(tpa ai))). *)
+          (*       { (* in same page *) *)
+          (*         iDestruct (pgt_big_sepM_split pgt Hlookup_ai with "[$pgt]") *)
+          (*           as "([_ p_instr] & Hacc_pgt)". *)
+          (*         iDestruct ("p_instr" with "[]") as (q_i) "[p_instr p_instr_q]";first done. *)
+          (*         iDestruct (mem_big_sepM_split_upd2 mem _ Hlookup_instr Hlookup_a_dst with "[$mem $Htotal_mem]") *)
+          (*           as "[a_instr [a_src Hacc_mem]]". *)
+          (*         iDestruct ("a_instr" with "[]") as "a_instr". *)
+          (*         { iPureIntro. exists (v, sacc).  split;done. } *)
+          (*         iDestruct ("a_src" with "[]") as "a_src". *)
+          (*         { iPureIntro. exists (v,sacc).  split. rewrite e1 //. simpl;done. } *)
+          (*         iApply (str_same_page ai a_dst src dst with "[PC p_instr a_instr a_src r_src r_dst rx]"); iFrameAutoSolve. *)
+          (*         { symmetry;done. } *)
+          (*         iNext. *)
+          (*         iIntros "(PC & a_instr & r_src & a_src & r_dst & p_instr & rx) _". *)
+          (*         iDestruct ("Hacc_regs" with "[$PC $r_src $r_dst]") as (regs') "[#Htotal_regs' regs]";iFrame. *)
+          (*         iDestruct ("Hacc_mem" with "[a_instr a_src]") as (mem') "[#Htotal_mem' mem]". *)
+          (*         { iSplitL "a_instr". *)
+          (*           iIntros "_". iFrame "a_instr". *)
+          (*           iIntros "_". iFrame "a_src". *)
+          (*         } *)
+          (*         iDestruct ("Hacc_pgt" with "[p_instr p_instr_q]") as "pgt". *)
+          (*         { iSplitL "". iIntros "%".  rewrite /= //in H. iIntros "_". iExists q_i. iFrame "p_instr p_instr_q". } *)
+          (*         iDestruct (VMProp_split with "VMProp") as "[VMProp1 VMProp2]". *)
+          (*         iSpecialize ("IH" $! pgt with "[regs Htotal_regs' rx tx VMProp1]"). *)
+          (*         iExists regs'. *)
+          (*         iFrame. *)
+          (*         iFrame "#". *)
+          (*         iExists p_rx. *)
+          (*         iFrame. *)
+          (*         iSpecialize ("IH" with "Hnotp"). *)
+          (*         iApply "IH". *)
+          (*         set Pred := (X in VMProp i X _). *)
+          (*         iExists Pred. *)
+          (*         iFrame. *)
+          (*         iNext. *)
+          (*         iLeft. *)
+          (*         iExists mem', shandle. *)
+          (*         iFrame. *)
+          (*         iFrame "#". *)
+          (*       } *)
+          (*       { (* in different pages *) *)
+          (*         (* getting pgt *) *)
+          (*         iDestruct (pgt_big_sepM_split2 pgt _ Hlookup_ai Hlookup_p_dst with "[$pgt]") *)
+          (*           as "([_ p_instr] & [_ p_src] & Hacc_pgt)". *)
+          (*         iDestruct ("p_instr" with "[]") as (q_i) "[p_instr p_instr_q]";first done. *)
+          (*         iDestruct ("p_src" with "[]") as (q_s) "[p_src p_src_q]";first done. *)
+          (*         (* getting mem *) *)
+          (*         rewrite /accessible_memory. *)
+          (*         iDestruct (mem_big_sepM_split_upd2 mem _ Hlookup_instr Hlookup_a_dst with "[$mem $Htotal_mem]") *)
+          (*           as "(a_instr & a_src & Hacc_mem)". *)
+          (*         iDestruct ("a_instr" with "[]") as "a_instr". *)
+          (*         { iPureIntro. exists (v,sacc).  split;done. } *)
+          (*         iDestruct ("a_src" with "[]") as "a_src". *)
+          (*         { iPureIntro. exists perm_dst.  split;done. } *)
+          (*         iApply (str ai a_dst src dst with "[PC p_instr p_src a_instr a_src r_src r_dst rx]"); iFrameAutoSolve. *)
+          (*         iNext. *)
+          (*         iIntros "(PC & a_instr & r_src & a_dst & r_dst & p_instr & p_src & rx) _". *)
+          (*         iDestruct ("Hacc_regs" with "[$PC $r_src $r_dst]") as (regs') "[#Htotal_regs' regs]";iFrame. *)
+          (*         iDestruct ("Hacc_mem" with "[a_instr a_dst]") as (mem') "[#Htotal_mem' mem]". *)
+          (*         { iSplitL "a_instr". *)
+          (*           iIntros "_". iFrame "a_instr". *)
+          (*           iIntros "_". iFrame "a_dst". *)
+          (*         } *)
+          (*         iDestruct ("Hacc_pgt" with "[p_instr p_instr_q p_src p_src_q]") as "pgt". *)
+          (*         { iSplitL "p_instr p_instr_q". iSplitL "". iIntros "%".  rewrite /= //in H. iIntros "_". iExists q_i. iFrame "p_instr p_instr_q". *)
+          (*           iSplitL "". iIntros "%".  rewrite /= //in H. iIntros "_". iExists q_s. iFrame "p_src p_src_q". } *)
+          (*         iDestruct (VMProp_split with "VMProp") as "[VMProp1 VMProp2]". *)
+          (*         iSpecialize ("IH" $! pgt with "[regs Htotal_regs' rx tx VMProp1]"). *)
+          (*         iExists regs'. *)
+          (*         iFrame. *)
+          (*         iFrame "#". *)
+          (*         iExists p_rx. *)
+          (*         iFrame. *)
+          (*         iSpecialize ("IH" with "Hnotp"). *)
+          (*         iApply "IH". *)
+          (*         set Pred := (X in VMProp i X _). *)
+          (*         iExists Pred. *)
+          (*         iFrame. *)
+          (*         iNext. *)
+          (*         iLeft. *)
+          (*         iExists mem', shandle. *)
+          (*         iFrame. *)
+          (*         iFrame "#". *)
+          (*       } *)
+          (*     } *)
+          (*   } *)
+          (* } *)
+          (* { (* no access to the page, apply ldr_error *) *)
+          (*   (* getting mem *) *)
+          (*   rewrite /accessible_memory. *)
+          (*   (* we don't update memory *) *)
+          (*   iDestruct (mem_big_sepM_split mem Hlookup_instr with "[$mem]") *)
+          (*     as "[instrm Hacc_mem]". *)
+          (*   iDestruct ("instrm" with "[]") as "a_instr". *)
+          (*   { iPureIntro. exists (v,sacc).  split;done. } *)
+          (*   (* getting pgt *) *)
+          (*   (* we don't update pagetable *) *)
+          (*   iDestruct (pgt_big_sepM_split2 pgt _ Hlookup_ai Hlookup_p_dst with "[$pgt]") *)
+          (*     as "([_ p_instr] & [p_dst _] & Hacc_pgt)". *)
+          (*   iDestruct ("p_instr" with "[]") as (q_i) "[p_instr p_instr_q]";first done. *)
+          (*   iDestruct ("p_dst" with "[]") as "p_dst";first done. *)
+          (*   iApply (str_no_access ai a_dst src dst with "[PC p_instr a_instr r_src r_dst p_dst]"); iFrameAutoSolve. *)
+          (*   iNext. *)
+          (*   iIntros "(PC & a_instr & r_src & p_src & r_dst) _". *)
+          (*   by iApply wp_terminated.             *)
+          (* } *)
         }
         { (* cmp: two cases *) admit. }
         { (* add *) admit. }
@@ -600,46 +597,50 @@ Section fundamental.
         { (* bne *) admit. }
         { (* br *) admit. }
         { (* halt *)
-          pose proof Heqn as Hdecode.
-          (* getting registers *)
-          iDestruct ((reg_big_sepM_split_upd regs i Hlookup_PC)
-                       with "[$Htotal_regs $regs]") as "(PC & Hacc_regs)".
-          iDestruct (pgt_big_sepM_split pgt Hlookup_ai with "[$pgt]")
-            as "[[_ p_instr] Hacc_pgt]".
-          rewrite /accessible_memory.
-          (* we don't update memory *)
-          iDestruct (mem_big_sepM_split mem Hlookup_instr with "[$mem]")
-            as "[instrm Hacc_mem]".
-          iDestruct ("instrm" with "[]") as "instrm".
-          { iPureIntro. exists (v,sacc).  split;done. }
-          iDestruct ("p_instr" with "[#]") as "(%q & p_instr & Hq)"; first done.
-          iApply (halt (s := {[i]}) (q := q) with "[PC p_instr instrm]"); iFrameAutoSolve.
-          set_solver.
-          iNext.
-          iIntros "? _".
-          by iApply wp_terminated.
+          admit.
+          (* pose proof Heqn as Hdecode. *)
+          (* (* getting registers *) *)
+          (* iDestruct ((reg_big_sepM_split_upd regs i Hlookup_PC) *)
+          (*              with "[$Htotal_regs $regs]") as "(PC & Hacc_regs)". *)
+          (* iDestruct (pgt_big_sepM_split pgt Hlookup_ai with "[$pgt]") *)
+          (*   as "[[_ p_instr] Hacc_pgt]". *)
+          (* rewrite /accessible_memory. *)
+          (* (* we don't update memory *) *)
+          (* iDestruct (mem_big_sepM_split mem Hlookup_instr with "[$mem]") *)
+          (*   as "[instrm Hacc_mem]". *)
+          (* iDestruct ("instrm" with "[]") as "instrm". *)
+          (* { iPureIntro. exists (v,sacc).  split;done. } *)
+          (* iDestruct ("p_instr" with "[#]") as "(%q & p_instr & Hq)"; first done. *)
+          (* iApply (halt (s := {[i]}) (q := q) with "[PC p_instr instrm]"); iFrameAutoSolve. *)
+          (* set_solver. *)
+          (* iNext. *)
+          (* iIntros "? _". *)
+          (* by iApply wp_terminated. *)
         }
         { (* fail *)
-          pose proof Heqn as Hdecode.
-          (* getting registers *)
-          iDestruct ((reg_big_sepM_split_upd regs i Hlookup_PC)
-                       with "[$Htotal_regs $regs]") as "(PC & Hacc_regs)".
-          iDestruct (pgt_big_sepM_split pgt Hlookup_ai with "[$pgt]")
-            as "[[_ p_instr] Hacc_pgt]".
-          rewrite /accessible_memory.
-          (* we don't update memory *)
-          iDestruct (mem_big_sepM_split mem Hlookup_instr with "[$mem]")
-            as "[instrm Hacc_mem]".
-          iDestruct ("instrm" with "[]") as "instrm".
-          { iPureIntro. exists (v,sacc).  split;done. }
-          iDestruct ("p_instr" with "[#]") as "(%q & p_instr & Hq)"; first done.
-          iApply (fail (s := {[i]}) (q := q) with "[PC p_instr instrm]"); iFrameAutoSolve.
-          set_solver.
-          iNext.
-          iIntros "? _".
-          by iApply wp_terminated.
+          admit.
+          (* pose proof Heqn as Hdecode. *)
+          (* (* getting registers *) *)
+          (* iDestruct ((reg_big_sepM_split_upd regs i Hlookup_PC) *)
+          (*              with "[$Htotal_regs $regs]") as "(PC & Hacc_regs)". *)
+          (* iDestruct (pgt_big_sepM_split pgt Hlookup_ai with "[$pgt]") *)
+          (*   as "[[_ p_instr] Hacc_pgt]". *)
+          (* rewrite /accessible_memory. *)
+          (* (* we don't update memory *) *)
+          (* iDestruct (mem_big_sepM_split mem Hlookup_instr with "[$mem]") *)
+          (*   as "[instrm Hacc_mem]". *)
+          (* iDestruct ("instrm" with "[]") as "instrm". *)
+          (* { iPureIntro. exists (v,sacc).  split;done. } *)
+          (* iDestruct ("p_instr" with "[#]") as "(%q & p_instr & Hq)"; first done. *)
+          (* iApply (fail (s := {[i]}) (q := q) with "[PC p_instr instrm]"); iFrameAutoSolve. *)
+          (* set_solver. *)
+          (* iNext. *)
+          (* iIntros "? _". *)
+          (* by iApply wp_terminated. *)
         }
-        { (* hvc *) admit. }
+        { (* hvc *)admit.
+          (*TODO*)
+        }
       }
       { (*invalid instruction *)
         iDestruct (reg_big_sepM_split regs i Hlookup_PC with "[$regs]") as "[PC _]".
