theories/rules/nop.v
@@ -1,5 +1,5 @@
 From machine_program_logic.program_logic Require Import weakestpre.
-From HypVeri.algebra Require Import base reg mem pagetable.
+From HypVeri.algebra Require Import base base_extra reg mem pagetable.
 From HypVeri Require Import machine_extra lifting rules.rules_base.
 From HypVeri.lang Require Import lang_extra reg_extra.
 
@@ -8,17 +8,18 @@ Section nop.
 Context `{hypparams: HypervisorParameters}.
 Context `{vmG: !gen_VMG Σ}.
 
-Lemma nop {E i w1 q } a :
+Lemma nop {E i w1 q s} a :
   decode_instruction w1 = Some Nop ->
+  (tpa a) ∈ s ->
   {SS{{ ▷ (PC @@ i ->r a)
         ∗ ▷ (a ->a w1)
-        ∗ ▷ ((tpa a) -@{ q }A> [{[i]}]) }}}
+        ∗ ▷ (i -@{ q }A> [s]) }}}
     ExecI @ i ; E
   {{{ RET (false, ExecI); (PC @@ i ->r (a ^+ 1)%f)
                   ∗ (a ->a w1)
-                  ∗ ((tpa a) -@{ q }A> [{[i]}]) }}}.
+                  ∗ (i -@{ q }A> [s])}}}.
 Proof.
-  iIntros (Hdecode ϕ) "(>Hpc & >Hapc & >Hacc) Hϕ".
+  iIntros (Hdecode Hin ϕ) "(>Hpc & >Hapc & >Hacc) Hϕ".
   iApply (sswp_lift_atomic_step ExecI);[done|].
   iIntros (n σ1) "%Hsche Hσ".
   rewrite /scheduled in Hsche.
@@ -34,16 +35,13 @@ Proof.
   (* valid regs *)
   iDestruct ((gen_reg_valid1 PC i a Hcur) with "Hreg Hpc") as "%HPC".
   (* valid pt *)
-  iDestruct (gen_access_valid σ1 with "Haccess Hacc") as %Hacc;eauto.
-  specialize (Hacc i).
+  iDestruct (access_agree_check_true with "Haccess Hacc") as %Hacc;first exact Hin.
   (* valid mem *)
   iDestruct (gen_mem_valid a w1 with "Hmem Hapc") as "%Hmem".
   iSplit.
   - (* reducible *)
     iPureIntro.
     eapply (reducible_normal i _ a w1); eauto.
-    apply Hacc.
-    set_solver +.
   - (* step *)
     iModIntro.
     iIntros (m2 σ2) "[%P PAuth] %HstepP".
@@ -53,7 +51,23 @@ Proof.
     destruct HstepP; subst m2 σ2; subst c2; simpl.
     rewrite /gen_vm_interp.
     (* unchanged part *)
-    rewrite_reg_pc.
+    rewrite (preserve_get_mb_gmap σ1).
+    rewrite (preserve_get_rx_gmap σ1).
+    rewrite (preserve_get_own_gmap σ1).
+    rewrite (preserve_get_access_gmap σ1).
+    rewrite (preserve_get_excl_gmap σ1).
+    rewrite (preserve_get_trans_gmap σ1).
+    rewrite (preserve_get_hpool_gset σ1).
+    rewrite (preserve_get_retri_gmap σ1).
+    rewrite (preserve_inv_trans_hpool_consistent σ1).
+    rewrite (preserve_inv_trans_pgt_consistent σ1).
+    rewrite (preserve_inv_trans_wellformed σ1).
+    rewrite (preserve_inv_pgt_mb_consistent σ1).
+    rewrite (preserve_inv_mb_wellformed σ1).
+    rewrite p_upd_pc_mem.
+    all: try rewrite p_upd_pc_pgt //.
+    all: try rewrite p_upd_pc_trans //.
+    all: try rewrite p_upd_pc_mb //.
     iFrame.
     (* updated part *)
     rewrite -> (update_offset_PC_update_PC1 _ i a 1); eauto.
@@ -71,7 +85,7 @@ Proof.
                   (seq 0 n) = []) as ->.
         {
           rewrite /scheduled /machine.scheduler //= /scheduler Hcur.
-          rewrite update_offset_PC_preserve_current_vm.
+          rewrite p_upd_pc_current_vm.
           rewrite Hcur.
           induction n.
           - simpl.
@@ -88,7 +102,7 @@ Proof.
         assert ((scheduled (update_offset_PC σ1 1) i) = true) as ->.
         {
           rewrite /scheduled /machine.scheduler //= /scheduler.
-          rewrite update_offset_PC_preserve_current_vm.
+          rewrite p_upd_pc_current_vm.
           rewrite Hcur.
           by case_bool_decide.
         }
@@ -96,7 +110,6 @@ Proof.
         iApply "Hϕ".
         iFrame.
     + solve_reg_lookup.
-    + apply Hacc;set_solver +.
 Qed.
 
 End nop.
